Got Core.Evaluate.fst written

src/Core.Environment.fst
@@ -16,12 +16,15 @@ The environment that typechecking occurs within.
 `ordmap` doesn't work with the `READER` effect,
 so I have to use something else. As such, I'm
 just falling back on a list.
+
+NOTE: look at the [FStar.DM4F.StMap](https://github.com/FStarLang/FStar/blob/master/examples/dm4free/FStar.DM4F.StMap.fst)
+example--it uses `FStar.Map` in a STATE monad.
 *)
 type env = list (name * decl)
 
 (** Look up a declaration within the typechecking
     environment. *)
-abstract val env_lookup : env -> name -> option decl
+abstract val env_lookup : env -> name -> Tot (option decl)
 let rec env_lookup e n =
   match e with
   | [] -> None
@@ -32,44 +35,19 @@ let rec env_lookup e n =
 (**
 `env_add` adds a declaration to an environment.
 *)
-abstract val env_add : env -> name -> decl -> env
+abstract val env_add : env -> name -> decl -> Tot env
 let env_add e n d = (n,d) :: e
 
 (**
 `env_init` initializes an environment using a
 list of tuples pairing a name and a declaration.
 *)
-abstract val env_init : list (name * decl) -> env
+abstract val env_init : list (name * decl) -> Tot env
 let env_init = id
 
-(** The base effect that typechecking occurs within. *)
-total reifiable reflectable new_effect TC = READER env
-
-(** Pre- and post-condition form for the `TC` effect. *)
-effect Tc (a:Type) (pre:TC?.pre) (post:env -> a -> GTot Type0) =
-  TC a (fun l0 p -> pre l0 /\ (forall x. pre l0 /\ post l0 x ==> p x))
-
-(** Utility effect for trivial conditions for the `TC` effect. *)
-effect TcNull (a:Type) =
-  TC a (fun (e0:env) (p:(a -> Type0)) -> forall (x:a). p x)
-
-(** Read the typechecking environment *)
-val read : unit -> TcNull env
-let read = TC?.get
-
-(** Lookup a declaration in the typechecking environment. *)
-val lookup : name -> TcNull (option decl)
-let lookup n =
-  let e = read () in
-  env_lookup e n
-
 (**
-Lookup the value associated with a name in the typechecking
-environment.
+Predicate for checking if a name is in the environment.
 *)
-val lookup_term : name -> TcNull (option ltt)
-let lookup_term n =
-  match lookup n with
-  | Some (Function t _) -> Some t
-  | _ -> None
-
+val env_has : env -> name -> Tot bool
+let rec env_has e n =
+  Option.isSome (env_lookup e n)
