src/Core.Evaluate.fst
@@ -1,0 +1,91 @@
+module Core.Evaluate
+
+open Core.Ltt
+open Core.Tc
+
+(** Notion of equality based on version3 of `pi-forall`.
+    
+    TODO: review this code; I think there are possible
+    problems, primarily with the way variables are handled--
+    in version3 `unbind2Plus` from the Unbound library
+    is used, and I'm not sure exactly what that's for.
+    
+    The other potential problem I see is just the fact
+    that I don't have a solid understanding of what
+    type theory I'm working under, which could introduce
+    subtle bugs. *)
+val equate : ltt -> ltt -> Tc unit
+let equate t1 t2 =
+  // if two terms have alpha equality they're
+  // equal.
+  if alpha_eq t1 t2 then () else 
+    let t1' = whnf t1 in
+    let t2' = whnf t2 in
+    let not_equal = CannotEquate t1' t2' in
+    match t1', t2' with
+    // Since we currently only have one Universe,
+    // they're trivially equal.
+    | Universe, Universe -> ()
+    
+    // Variables are equal if the names are equal.
+    //
+    // TODO: figure out if this is going to cause
+    // bugs. Hopefully the check for alpha equality
+    // should ensure that this only comes up if both
+    // variables are free.
+    | Var x, Var y -> require (x = y)
+
+    // Applications are equal if the left and right
+    // sides are equal.
+    | App l1 r1, App l2 r2 ->
+      equate l1 l2;
+      equate r1 r2
+
+    // Equality of abstractions depends on the binding.
+    | Abs bnd1 v1 tm1, Abs bnd2 v2 tm2 ->
+      match bnd1, bnd2 with
+      // Lambdas are equal if the bodies are equal.
+      //
+      // >>> \x.e = \y.e
+      | Lam, Lam -> equate tm1 tm2
+
+      // Pis are the same if the types are the equal
+      // and the bodies are the equal.
+      //
+      // >>> (x:A) -> B = (y:A) -> B
+      | Pi ty1, Pi ty2 ->
+        equate ty1 ty2;
+        equate tm1 tm2
+
+      // If neither matches, the abstractions are
+      // not equal.
+      | _ -> raise not_equal
+
+    // If none of these cases match, the terms are
+    // not equal.
+    | _ -> raise not_equal
+
+(** Assert that a value is a function type. *)
+val ensurePi : ltt -> Tc (ty: ltt * var: name * body: ltt)
+let ensurePi t =
+  let t' = whnf t in
+  match t' with
+  | Abs (Pi ty) var body -> ty * var * body
+  | _ -> raise (ExpectedFunctionType t)
+
+(** Put a term into weak head normal form.
+    
+    Based on version3 of `pi-forall`. *)
+val whnf : ltt -> Tc ltt
+let rec whnf t =
+  match t with
+  | Var n ->
+    match lookup_def n with
+    | Some v -> v
+    | None -> t
+  | App l r ->
+    match l with
+    | Abs Lam v body ->
+      whnf (subst r v body)
+    | _ -> t
+  | _ -> t
