src/Core.Tc.fst
@@ -1,0 +1,127 @@
+module Core.Tc
+open Core.Ltt
+open Core.Environment
+
+(** Representation of a type checking error. *)
+type tc_err =
+  | MissingDeclFor : name -> tc_err
+  | CannotEquate : ltt -> ltt -> tc_err
+  | ExpectedFunctionType : ltt -> tc_err
+  | Msg : string -> tc_err
+
+(** The result of a type checking operation: either a
+    success (`Ok`) or a failure (`Err`). *)
+type tc_result 'a =
+  | Err : tc_err -> tc_result 'a
+  | Ok : 'a -> tc_result 'a
+
+(** Internal representation of the tc monad. *)
+private let tc (a:Type) = env -> M (tc_result a)
+
+(** Lift a value `x` into the tc monad. *)
+private val return_tc : a:Type -> a -> Tot (tc a)
+let return_tc _ x = fun _ -> Ok x
+
+(** Bind a function in the tc monad. *)
+private val bind_tc : a:Type -> b:Type
+                    -> x:tc a -> f:(a -> tc b) -> Tot (tc b)
+let bind_tc _ _ x f =
+  fun env ->
+    let res = x env in
+    match res with
+    | Ok v -> f v env
+    | Err err -> Err err
+
+(** Implementation of the `raise` action in the tc monad. *)
+private val tc_raise : a:Type -> tc_err -> Tot (tc a)
+let tc_raise a err: tc a = fun _ -> Err err
+
+(** Implementation of the `get` action in the tc monad. *)
+private val tc_get : unit -> Tot (tc env)
+let tc_get (): tc env = fun envr -> Ok envr
+
+(** Definition of the `TC` effect. *)
+total reifiable reflectable new_effect {
+  TC : a:Type -> Effect
+  with repr   = tc
+     ; bind   = bind_tc
+     ; return = return_tc
+     ; get    = tc_get
+     ; raise  = tc_raise
+}
+
+(** Pre- and post-condition form for the `TC` effect. *)
+effect Tc (a:Type) (pre:TC?.pre) (post:env -> tc_result a -> GTot Type0) =
+  TC a
+    (fun (envr:env) (p:TC?.post a) ->
+      pre envr /\
+        (forall (r:tc_result a). pre envr /\ post envr r ==> p r))
+
+(** Utility effect for trivial conditions for the `TC` effect. *)
+effect TcNull (a:Type) =
+  TC a (fun (e0:env) (p:(a -> Type0)) -> forall (x:a). p x)
+
+(** Get the typechecking environment. *)
+val get : unit -> TcNull env
+let get = TC?.get
+
+(** Raise a typechecking error. *)
+val raise : (#a:Type) -> err:tc_err -> Tc a
+  (requires fun _ -> True)
+  (ensures fun _ r -> r = Err err)
+let raise #a err = TC?.raise a err
+
+(** Specification of the behavior of `unwrap_opt`. *)
+private val unwrap_opt_spec : tc_err -> option 'a -> tc_result 'a -> Type0
+let unwrap_opt_spec err o r =
+  match r with
+  | Ok v -> o = Some v
+  | Err err' -> o = None /\ err' = err
+
+(** Unwrap an `option`, and if it's `None` raise the passed error. *)
+val unwrap_opt : err:tc_err -> o:option 'a -> Tc 'a
+  (requires fun _ -> True)
+  (ensures fun _ r -> unwrap_opt_spec err o r)
+let unwrap_opt err o =
+  match o with
+  | Some v -> v
+  | None -> raise err
+
+(** A form of runtime assert that raises `err` if `b = false`. *)
+val require : err:tc_err -> b:bool -> Tc unit
+  (ensures fun _ -> True)
+  (requires fun _ r -> if b
+    then r = Ok ()
+    else r = Err err)
+let require err b =
+  if b then () else raise err
+
+(** Lookup a declaration in the typechecking environment. *)
+val lookup : name -> TcNull (option decl)
+let lookup n =
+  let e = get () in
+  env_lookup e n
+
+(** Lookup the value associated with a name in the typechecking
+    environment. *)
+val lookup_def : name -> TcNull (option ltt)
+let lookup_def n =
+  match lookup n with
+  | Some (Function t _) -> Some t
+  | _ -> None
+
+(** Specification of the behavior of `lookup'`. *)
+val lookup'_spec : env -> name -> tc_result decl -> Type0
+let lookup'_spec envr n r =
+  match r with
+  | Ok v -> env_lookup envr n = Some v
+  | Err _ -> env_lookup envr n = None
+
+(** Unwrapped version of `lookup` that raises an error
+    if `n` is not in the typechecking environment. *)
+val lookup' : n:name -> Tc decl
+  (requires fun envr -> True)
+  (ensures fun e r -> lookup'_spec e n r)
+let lookup' n =
+  let o = lookup n in
+  unwrap_opt (MissingDeclFor n) o
