TODO.md
@@ -1,4 +1,3 @@
 # TODO
-1. add `Exn` to the `Tc` monad
-2. implement weak head normal form
-3. implement `equate`
+1. Implement runTc
+2. Implement typecheck
